feat: add List/Array/Vector.ofFnM

src/Init/Data/Array/OfFn.lean
@@ -9,6 +9,7 @@ prelude
 import all Init.Data.Array.Basic
 import Init.Data.Array.Lemmas
 import Init.Data.List.OfFn
+import Init.Data.List.FinRange
 
 /-!
 # Theorems about `Array.ofFn`
@@ -17,7 +18,41 @@ import Init.Data.List.OfFn
 set_option linter.listVariables true -- Enforce naming conventions for `List`/`Array`/`Vector` variables.
 set_option linter.indexVariables true -- Enforce naming conventions for index variables.
 
+namespace List
+
+/-! ### ofFnM
+
+We prove some theorems about `List.ofFnM` here, as they rely on `Array` lemmas.
+-/
+
+theorem ofFnM_succ {n} [Monad m] [LawfulMonad m] {f : Fin (n + 1) → m α} :
+    ofFnM f = (do
+      let a ← f 0
+      let as ← ofFnM fun i => f i.succ
+      pure (a :: as)) := by
+  simp [ofFnM, Fin.foldlM_eq_finRange_foldlM, List.foldlM_push_eq_append, List.finRange_succ, Function.comp_def]
+
+theorem ofFnM_succ_last {n} [Monad m] [LawfulMonad m] {f : Fin (n + 1) → m α} :
+    ofFnM f = (do
+      let as ← ofFnM fun i => f i.castSucc
+      let a  ← f (Fin.last n)
+      pure (as ++ [a])) := by
+  simp [ofFnM, Fin.foldlM_succ_last]
+
+theorem ofFnM_add {n m} [Monad m] [LawfulMonad m] {f : Fin (n + k) → m α} :
+    ofFnM f = (do
+      let as ← ofFnM fun i : Fin n => f (i.castLE (Nat.le_add_right n k))
+      let bs ← ofFnM fun i : Fin k => f (i.natAdd n)
+      pure (as ++ bs)) := by
+  induction k with
+  | zero => simp
+  | succ k ih => simp [ofFnM_succ_last, ih]
+
+end List
+
 namespace Array
+
+/-! ### ofFn -/
 
 @[simp] theorem ofFn_zero {f : Fin 0 → α} : ofFn f = #[] := by
   simp [ofFn, ofFn.go]
@@ -33,11 +68,22 @@ theorem ofFn_succ {f : Fin (n+1) → α} :
       simp at h₁ h₂
       omega
 
+theorem ofFn_add {n m} {f : Fin (n + m) → α} :
+    ofFn f = (ofFn (fun i => f (i.castLE (Nat.le_add_right n m)))) ++ (ofFn (fun i => f (i.natAdd n))) := by
+  induction m with
+  | zero => simp
+  | succ m ih => simp [ofFn_succ, ih]
+
 @[simp] theorem _root_.List.toArray_ofFn {f : Fin n → α} : (List.ofFn f).toArray = Array.ofFn f := by
   ext <;> simp
 
 @[simp] theorem toList_ofFn {f : Fin n → α} : (Array.ofFn f).toList = List.ofFn f := by
   apply List.ext_getElem <;> simp
+
+theorem ofFn_succ' {f : Fin (n+1) → α} :
+    ofFn f = #[f 0] ++ ofFn (fun i => f i.succ) := by
+  apply Array.toList_inj.mp
+  simp [List.ofFn_succ]
 
 @[simp]
 theorem ofFn_eq_empty_iff {f : Fin n → α} : ofFn f = #[] ↔ n = 0 := by
@@ -52,5 +98,53 @@ theorem mem_ofFn {n} {f : Fin n → α} {a : α} : a ∈ ofFn f ↔ ∃ i, f i =
     exact ⟨⟨i, by simpa using h⟩, by simp⟩
   · rintro ⟨i, rfl⟩
     apply mem_of_getElem (i := i) <;> simp
+
+/-! ### ofFnM -/
+
+/-- Construct (in a monadic context) an array by applying a monadic function to each index. -/
+def ofFnM {n} [Monad m] (f : Fin n → m α) : m (Array α) :=
+  Fin.foldlM n (fun xs i => xs.push <$> f i) (Array.mkEmpty n)
+
+@[simp]
+theorem ofFnM_zero [Monad m] {f : Fin 0 → m α} : ofFnM f = pure #[] := by
+  simp [ofFnM]
+
+theorem ofFnM_succ' {n} [Monad m] [LawfulMonad m] {f : Fin (n + 1) → m α} :
+    ofFnM f = (do
+      let a ← f 0
+      let as ← ofFnM fun i => f i.succ
+      pure (#[a] ++ as)) := by
+  simp [ofFnM, Fin.foldlM_eq_finRange_foldlM, List.foldlM_push_eq_append, List.finRange_succ, Function.comp_def]
+
+theorem ofFnM_succ {n} [Monad m] [LawfulMonad m] {f : Fin (n + 1) → m α} :
+    ofFnM f = (do
+      let as ← ofFnM fun i => f i.castSucc
+      let a  ← f (Fin.last n)
+      pure (as.push a)) := by
+  simp [ofFnM, Fin.foldlM_succ_last]
+
+theorem ofFnM_add {n m} [Monad m] [LawfulMonad m] {f : Fin (n + k) → m α} :
+    ofFnM f = (do
+      let as ← ofFnM fun i : Fin n => f (i.castLE (Nat.le_add_right n k))
+      let bs ← ofFnM fun i : Fin k => f (i.natAdd n)
+      pure (as ++ bs)) := by
+  induction k with
+  | zero => simp
+  | succ k ih =>
+    simp only [ofFnM_succ, Nat.add_eq, ih, Fin.castSucc_castLE, Fin.castSucc_natAdd, bind_pure_comp,
+      bind_assoc, bind_map_left, Fin.natAdd_last, map_bind, Functor.map_map]
+    congr 1
+    funext xs
+    congr 1
+    funext ys
+    congr 1
+    funext x
+    simp
+
+@[simp] theorem toList_ofFnM [Monad m] [LawfulMonad m] {f : Fin n → m α} :
+    toList <$> ofFnM f = List.ofFnM f := by
+  induction n with
+  | zero => simp
+  | succ n ih => simp [ofFnM_succ, List.ofFnM_succ_last, ← ih]
 
 end Array
